CommitmentSpecial.ec
@@ -1,0 +1,29 @@
+require import AllCore Distr.
+
+
+type commitment, opening, message.
+
+
+op Com  : message -> (commitment * opening) distr.
+op Ver : message * (commitment * opening) -> bool.
+
+axiom Com_sound : forall (x : message * (commitment * opening)), x.`2 \in Com x.`1 => Ver x.
+axiom Com_lossless : forall b, is_lossless (Com b).
+
+
+module type Binder = {
+   proc bind() : commitment * message * opening * message * opening
+}.
+
+module BindingExperiment (B:Binder) = {
+    proc main() : bool = {
+      var c, m, m', d, d', v, v';
+
+      (* x                 <@ S.gen(); *)
+      (c, m, d, m', d') <@ B.bind();
+      v                 <- Ver (m, (c, d));
+      v'                <- Ver (m', (c, d'));
+
+      return v /\ v' /\ m <> m';
+    }
+}.
