HC/Completeness.ec
@@ -1,0 +1,188 @@
+pragma Goals:printall.
+require import AllCore DBool Bool List Distr Int Aux DJoin.
+
+require import Permutation Basics.
+
+axiom kjk prm n w : prm \in perm_d n =>
+ uniq w => (forall i, i \in w => 0 <= i < n) =>
+  size w = n => uniq (permute_wit prm w).
+
+axiom prj_lemma (g : graph) (w : hc_wit) (perm : permutation) : 
+  take (size w) (ip (prj w) g) 
+  = take (size w) (ip (prj (permute_wit perm w)) (fap perm g)).
+
+
+section.
+
+local lemma hc_complete_hoare pa wa : IsHC (pa,wa) =>
+   hoare[ Completeness(HonestProver, HonestVerifier).run : arg = (pa,wa) ==> res ].
+move => ishc. proc. inline*. wp. rnd. 
+wp. rnd. wp. rnd. wp. skip.
+progress.
+pose b1 := challenge00.
+
+case (b1 = true). 
+move => h. rewrite h. simplify.
+  + have ->: (zip (unzip1 x0) (unzip2 x0)) = x0. rewrite zip_unzip. auto.
+split.
+have : all (fun (xy : bool * (commitment * opening) ) => xy.`2 \in (Com xy.`1)) 
+    (zip  (fap prm statement{hr}.`2) x0).
+have f3 :   
+  size (fap prm statement{hr}.`2) = size x0 /\
+  all (fun (xy : bool * (commitment * opening)) => xy.`2 \in Com xy.`1)
+    (zip (fap prm statement{hr}.`2) x0).
+apply (supp_djoinmap Com ((fap prm statement{hr}.`2))  x0). auto.
+elim f3. move => f31 f32.
+auto.
+move => q.
+apply (sub_all (fun (xy : bool * (commitment * opening)) => xy.`2 \in Com xy.`1) Ver) .
+simplify. apply Com_sound.  auto.
+have f1 : size x0 = size (fap prm statement{hr}.`2).
+smt.
+have f2 : size x0 = size (unzip1 x0).
+smt.
+rewrite - f2. 
+rewrite f1.
+rewrite fap_prop2.
+split. smt. split. smt. smt.
+move => p.
+have ->: b1 = false. smt.
+simplify. clear p. progress.
+apply (kjk prm statement{hr}.`1). auto. smt (ishc_prop4). smt (ishc_prop4).
+smt. 
+smt.
+have ->: size (unzip1 x0) = size x0. smt.
+have -> : size x0 = size (fap prm statement{hr}.`2). smt(supp_djoinmap).
+have -> : size (fap prm statement{hr}.`2) = size (statement{hr}.`2). smt. smt.
+have ->: size (unzip2 (take statement{hr}.`1 (ip (prj (permute_wit prm witness{hr})) x0)))
+ = size (take statement{hr}.`1 (ip (prj (permute_wit prm witness{hr})) x0)). smt.
+have : statement{hr}.`1 <= size (ip (prj (permute_wit prm witness{hr})) x0).
+have ->: size (ip (prj (permute_wit prm witness{hr})) x0) = size x0.
+smt.
+have -> : size x0 = size (fap prm statement{hr}.`2). smt(supp_djoinmap).
+have -> : size (fap prm statement{hr}.`2) = size (statement{hr}.`2). smt. timeout 20. smt.
+progress. smt.
+have ->: 
+  (unzip2 (take statement{hr}.`1 (ip (prj (permute_wit prm witness{hr})) x0)))
+  = ((take statement{hr}.`1 (unzip2 (ip (prj (permute_wit prm witness{hr})) x0)))).
+smt.
+have ->: 
+  (zip (take statement{hr}.`1 (ip (prj (permute_wit prm witness{hr})) (unzip1 x0)))
+     (take statement{hr}.`1 (unzip2 (ip (prj (permute_wit prm witness{hr})) x0))))
+  = take statement{hr}.`1  
+     (zip ((ip (prj (permute_wit prm witness{hr})) (unzip1 x0)))
+          ((unzip2 (ip (prj (permute_wit prm witness{hr})) x0)))).
+apply take_zip.
+have ->: ((ip (prj (permute_wit prm witness{hr})) (unzip1 x0)))
+  = (unzip1 (ip (prj (permute_wit prm witness{hr})) (x0))).
+rewrite map_ip. auto.
+have ->: 
+ (zip (unzip1 (ip (prj (permute_wit prm witness{hr})) x0))
+        (unzip2 (ip (prj (permute_wit prm witness{hr})) x0)))
+ = (ip (prj (permute_wit prm witness{hr})) x0).
+apply zip_unzip.
+pose pi_w := (permute_wit prm witness{hr}).
+pose n := statement{hr}.`1.
+pose fapg := (fap prm statement{hr}.`2). 
+have ->: 
+ all Ver (zip (nseq n true) (take n (ip (prj pi_w) x0)))
+ = all (fun x => Ver x)
+  (take n (zip (nseq n true) (ip (prj pi_w) x0))).
+rewrite - take_zip.
+rewrite take_nseq. auto.
+have ->: (take n (zip (nseq n true) (ip (prj pi_w) x0))) =
+  (take n (zip (ip (prj pi_w) fapg) (ip (prj pi_w) x0))).
+  have ->: take n (zip (nseq n true) (ip (prj pi_w) x0)) =
+     (zip (nseq n true) (ip (prj pi_w) x0)). 
+apply take_oversize.
+rewrite size_zip.
+rewrite size_nseq. 
+  have ->: (max 0 n) = n.  smt(ishc_prop2). smt.
+  have ->: take n (zip (ip (prj pi_w) fapg) (ip (prj pi_w) x0))
+   = (zip (take n (ip (prj pi_w) fapg)) (take n (ip (prj pi_w) x0))).
+   rewrite - take_zip. auto.
+  have ->: (take n (ip (prj pi_w) fapg)) = nseq n true.
+  rewrite - (ishc_prop3 (statement{hr}, witness{hr}) statement{hr}.`1 statement{hr}.`2 witness{hr}). auto. smt. rewrite /n.
+  have ->: statement{hr}.`1 = size (witness{hr}). smt. rewrite -  prj_lemma. auto.   
+rewrite - take_nseq.
+rewrite take_zip.
+rewrite take_nseq.
+rewrite take_oversize.
+rewrite size_zip.
+rewrite size_nseq. 
+  have ->: (max 0 n) = n.  smt(ishc_prop2). smt.
+auto.   
+have f1 : all Ver (zip fapg x0). 
+search djoin.
+  have :   size (fap prm statement{hr}.`2) = size x0 /\ all (fun xy => snd xy \in Com xy.`1) (zip fapg x0).
+   apply (supp_djoinmap Com fapg x0 ). apply H0.
+   elim. progress.
+  have : forall x, x \in (zip fapg x0) => x.`2 \in Com x.`1.
+apply allP. apply H3.
+progress.
+apply allP. progress. 
+  have : x1.`2 \in Com x1.`1. apply H4. auto.
+  apply Com_sound.
+have f2 : all Ver (zip (ip (prj pi_w) fapg)  (ip (prj pi_w) x0)).
+rewrite - zip_ip.
+have : forall x, x \in (zip fapg x0) => Ver x.
+apply allP. apply f1.
+progress.
+have : forall x, x \in (ip (prj pi_w) (zip fapg x0)) => Ver x.
+progress. apply H2.
+  have ff : perm_eq (zip fapg x0) (ip (prj pi_w) (zip fapg x0)).
+   smt.
+  smt.
+apply allP.
+timeout 20. smt.
+rewrite /permute_wit.
+elim ishc. progress.
+have : perm_eq (map prm witness{hr}) (map prm (range 0 statement{hr}.`1)).
+smt.
+progress.
+have : perm_eq (map prm (range 0 statement{hr}.`1)) (range 0 statement{hr}.`1).
+smt.
+smt.
+smt.
+qed.
+
+local lemma djoinmap_weight (d : 'a -> 'b distr) :  forall l,
+  (forall x, is_lossless (d x)) =>
+    weight (djoinmap d l) = 1%r.
+elim. smt (weight_djoin_nil).
+smt (weight_djoin_cons).
+qed.
+
+local lemma hc_complete statement witness &m : IsHC (statement,witness) =>
+  Pr[Completeness(HonestProver, HonestVerifier).run(statement, witness) @ &m : true] = 1%r.
+move => inlang. byphoare (_: arg = (statement, witness) ==> _);auto. proc. inline*. wp. rnd.  simplify. wp. 
+rnd.  wp. 
+conseq (_: _ ==> true). progress. smt (@Distr @DBool). 
+apply djoinmap_weight. apply Com_lossless.
+rnd. wp.  skip. progress. apply perm_d_lossless. smt (ishc_prop2). 
+qed.
+
+
+local lemma hc_complete_failure statement witness &m : IsHC (statement,witness) =>
+     Pr[Completeness(HonestProver, HonestVerifier).run(statement, witness) @ &m : !res] = 0%r.
+progress. byphoare (_: arg = (statement,witness) ==> _);auto.
+hoare. simplify. conseq (hc_complete_hoare statement witness H).
+qed.
+
+
+lemma hc_completeness: forall (statement : hc_prob) (witness : int list) &m,
+        IsHC (statement, witness) =>
+     Pr[Completeness(HonestProver, HonestVerifier).run(statement, witness) 
+            @ &m : res] = 1%r.
+progress. 
+rewrite - (hc_complete statement witness &m H).
+have f : 0%r = 
+ Pr[Completeness(HonestProver, HonestVerifier).run(statement, witness) @ &m : true]
+  - Pr[Completeness(HonestProver, HonestVerifier).run(statement, witness) @ &m : res].
+rewrite Pr[mu_split res].  
+rewrite hc_complete_failure;auto. 
+smt.
+qed.
+
+end section.
+
